take out the more generic language-with-db-indices stuff

theories/examples/affine.v
@@ -1,8 +1,84 @@
 (** Affine functions *)
 From Equations Require Import Equations.
 From gitrees Require Import gitree program_logic.
-From gitrees.input_lang Require Import lang interp logrel.
+From gitrees.input_lang Require Import lang interp.
 From gitrees.examples Require Import store pairs.
+
+Module io_lang.
+  Definition ty := input_lang.lang.ty.
+  Definition expr := input_lang.lang.expr.
+  Definition typed {S} := input_lang.lang.typed (S:=S).
+  Definition interp_closed {sz} (rs : gReifiers sz) `{!subReifier reify_io rs} (e : expr []) := input_lang.interp.interp_expr rs e ().
+End io_lang.
+
+Inductive ty :=
+  tBool | tInt | tUnit
+| tArr (τ1 τ2 : ty) | tPair (τ1 τ2 : ty).
+
+Inductive expr : scope → Type :=
+| LitBool (b : bool) {S} : expr S
+| LitNat (n : nat) {S} : expr S
+| LitUnit {S} : expr S
+| Lam {S} : expr (tt::S) → expr S
+| Var {S} : var S → expr S
+| App {S1 S2} : expr S1 → expr S2 → expr (S1++S2)
+(* | EPair {S} : expr S → expr S → expr S *)
+(* | EDestruct {S} : expr S → expr (()::()::S) → expr S *)
+| EEmbed {S} : io_lang.expr [] → expr S
+.
+
+Local Notation tyctx := (tyctx ty).
+Inductive typed : forall {S}, tyctx  S → expr S → ty → Prop :=
+| typed_Var {S} (Ω : tyctx S) (τ : ty) (v : var S)  :
+  typed_var Ω v τ →
+  typed Ω (Var v) τ
+| typed_Lam {S} (Ω : tyctx S) (τ1 τ2 : ty) (e : expr (()::S) ) :
+  typed (consC τ1 Ω) e τ2 →
+  typed Ω (Lam e) (tArr τ1 τ2)
+| typed_App {S1 S2} (Ω1 : tyctx S1) (Ω2 : tyctx S2) (τ1 τ2 : ty) e1 e2 :
+  typed Ω1 e1 (tArr τ1 τ2) →
+  typed Ω2 e2 τ1 →
+  typed (tyctx_app Ω1 Ω2) (App e1 e2) τ2
+| typed_Nat {S} (Ω : tyctx S) n :
+  typed Ω (LitNat n) tInt
+| typed_Bool {S} (Ω : tyctx S) b :
+  typed Ω (LitBool b) tBool
+| typed_Unit {S} (Ω : tyctx S) :
+  typed Ω LitUnit tUnit
+.
+
+Inductive ty_conv : ty → input_lang.lang.ty → Type :=
+| ty_conv_bool : ty_conv tBool Tnat
+| ty_conv_int  : ty_conv tInt  Tnat
+| ty_conv_unit : ty_conv tUnit Tnat
+| ty_conv_fun {τ1 τ2 t1 t2} :
+  ty_conv τ1 t1 → ty_conv τ2 t2 →
+  ty_conv (tArr τ1 τ2) (Tarr (Tarr Tnat t1) t2)
+.
+
+
+Module iolang.
+  Context {sz : nat}.
+  Variable rs : gReifiers sz.
+  Context `{!subReifier reify_io rs}.
+  Notation F := (gReifiers_ops rs).
+  Notation IT := (IT F).
+  Notation ITV := (ITV F).
+  Context `{!invGS Σ, !stateG rs Σ}.
+  Notation iProp := (iProp Σ).
+
+  Variable s : stuckness.
+
+  Program Definition interp_tnat : ITV -n> iProp := λne αv,
+    (∃ n, αv ≡ NatV n)%I.
+  Solve All Obligations with solve_proper.
+  Program Definition interp_tarr (Φ1 Φ2 : ITV -n> iProp) := λne αv,
+    (□ ∀ βv, Φ1 βv -∗ WP@{rs} IT_of_V αv ⊙ (IT_of_V βv) @ s {{ Φ2 }})%I.
+  Solve All Obligations with solve_proper.
+
+End iolang.
+
+Definition s : stuckness := λ e, e = OtherError.
 
 Section affine.
   Context {sz : nat}.
@@ -32,10 +108,6 @@ Section affine.
   Solve All Obligations with first [solve_proper|solve_proper_please].
   Program Definition Force : IT -n> IT := λne e, e ⊙ (Nat 0).
 
-  Inductive ty :=
-     tBool | tInt | tUnit
-   | tArr (τ1 τ2 : ty) | tPair (τ1 τ2 : ty).
-
   Local Open Scope type.
   Definition interp_litbool (b : bool) {A} : A -n> IT := λne _,
     Nat (if b then 1 else 0).
@@ -51,20 +123,43 @@ Section affine.
   Solve All Obligations with solve_proper_please.
   Program Definition interp_app {A1 A2 : ofe} (t1 : A1 -n> IT) (t2 : A2 -n> IT)
     : A1*A2 -n> IT := λne env,
-    APP' (t1 env.1) (LET (t2 env.2) Thunk).
+    LET (t2 env.2) $ λne x,
+    LET (t1 env.1) $ λne f,
+    APP' f (Thunk x).
   Solve All Obligations with solve_proper_please.
-  Program Definition interp_destruct {A1 A2 : ofe}
-       (ps : A1 -n> IT) (t : IT*IT*A2 -n> IT)
-    : A1*A2 -n> IT := λne env,
-    LET (ps env.1) $ λne ps,
-    LET (Thunk (proj1T ps)) $ λne x,
-    LET (Thunk (proj2T ps)) $ λne y,
-    t (x, y, env.2).
-  Solve All Obligations with solve_proper_please.
+  (* Program Definition interp_destruct {A1 A2 : ofe} *)
+  (*      (ps : A1 -n> IT) (t : IT*IT*A2 -n> IT) *)
+  (*   : A1*A2 -n> IT := λne env, *)
+  (*   LET (ps env.1) $ λne ps, *)
+  (*   LET (Thunk (proj1T ps)) $ λne x, *)
+  (*   LET (Thunk (proj2T ps)) $ λne y, *)
+  (*   t (x, y, env.2). *)
+  (* Solve All Obligations with solve_proper_please. *)
+
+  Definition interp_scope_split {S1 S2} {E} :
+    interp_scope (E:=E) (S1 ++ S2) -n> interp_scope (E:=E) S1 * interp_scope (E:=E) S2.
+  Proof.
+    induction S1 as [|? S1]; simpl.
+    - simple refine (λne x, (tt, x)).
+      solve_proper.
+    - simple refine (λne xy, let ss := IHS1 xy.2 in ((xy.1, ss.1), ss.2)).
+      solve_proper.
+  Defined.
+
+  Fixpoint interp_expr {S} (e : expr S) : interp_scope S -n> IT :=
+    match e with
+    | LitBool b => interp_litbool b
+    | LitNat n  => interp_litnat n
+    | LitUnit   => interp_litunit
+    | Var v     => interp_var v
+    | Lam e    => interp_lam (interp_expr e)
+    | App e1 e2 => interp_app (interp_expr e1) (interp_expr e2) ◎ interp_scope_split
+    | EEmbed io_expr => constO (io_lang.interp_closed rs io_expr)
+    end.
 
   (* interpreting tys *)
   Program Definition protected (Φ : ITV -n> iProp) : ITV -n> iProp := λne αv,
-    (WP@{rs} Force (IT_of_V αv) {{ Φ }})%I.
+    (WP@{rs} Force (IT_of_V αv) @ s {{ Φ }})%I.
   Solve All Obligations with solve_proper_please.
   Program Definition interp_tbool : ITV -n> iProp := λne αv,
     (αv ≡ NatV 0 ∨ αv ≡ NatV 1)%I.
@@ -80,8 +175,8 @@ Section affine.
                        Φ1 β1v ∗ Φ2 β2v)%I.
   Solve All Obligations with solve_proper_please.
   Program Definition interp_tarr (Φ1 Φ2 : ITV -n> iProp) : ITV -n> iProp := λne αv,
-    (∀ βv l, Φ1 βv -∗ pointsto l (Nat 0) -∗
-             WP@{rs} ((IT_of_V αv) ⊙ (thunked (IT_of_V βv) l)) {{ Φ2 }})%I.
+    (∀ βv, Φ1 βv -∗
+             WP@{rs} ((IT_of_V αv) ⊙ (Thunk (IT_of_V βv))) @ s {{ Φ2 }})%I.
   Solve All Obligations with solve_proper_please.
 
   Fixpoint interp_ty (τ : ty) : ITV -n> iProp :=
@@ -93,148 +188,188 @@ Section affine.
     | tArr τ1 τ2  => interp_tarr  (interp_ty τ1) (interp_ty τ2)
     end.
 
-  Lemma compat_bool b {A :ofe} (e : A) :
-    ⊢ WP@{rs} (interp_litbool b e) {{ interp_tbool }}.
+  Definition ssubst_valid {S} (Ω : tyctx S) (ss : ssubst S) : iProp :=
+    ([∗ list] τx ∈ zip (list_of_tyctx Ω) (list_of_ssubst (E:=F) ss),
+      interp_ty (τx.1) (τx.2))%I.
+
+  Definition valid1 {S} (Ω : tyctx S) (α : interp_scope S -n> IT) (τ : ty) : iProp :=
+    ∀ ss, ssubst_valid Ω ss -∗ heap_ctx -∗ WP@{rs} α (interp_ssubst ss) @ s {{ interp_ty τ }}.
+
+  Lemma compat_bool {S} b (Ω : tyctx S) :
+    ⊢ valid1 Ω (interp_litbool b) tBool.
   Proof.
+    iIntros (αs) "Has #Hctx".
     simpl. iApply wp_val. iModIntro.
     destruct b; simpl; eauto.
   Qed.
-  Lemma compat_nat n {A :ofe} (e : A) :
-    ⊢ WP@{rs} (interp_litnat n e) {{ interp_tnat }}.
+  Lemma compat_nat {S} n (Ω : tyctx S) :
+    ⊢ valid1 Ω (interp_litnat n) tInt.
   Proof.
+    iIntros (αs) "Has #Hctx".
     simpl. iApply wp_val. iModIntro. eauto.
   Qed.
-  Lemma compat_unit {A :ofe} (e : A) :
-    ⊢ WP@{rs} (interp_litunit e) {{ interp_tunit }}.
+  Lemma compat_unit {S} (Ω : tyctx S) :
+    ⊢ valid1 Ω interp_litunit tUnit.
   Proof.
+    iIntros (αs) "Has #Hctx".
     simpl. iApply wp_val. iModIntro. eauto.
-  Qed.
-  Lemma compat_pair {A1 A2 : ofe} (e1 : A1) (e2 : A2) (Φ1 Φ2 : ITV -n> iProp)
-    (α : A1 -n> IT) (β : A2 -n> IT) :
-    heap_ctx ⊢ WP@{rs} α e1 {{ Φ1 }} -∗
-               WP@{rs} β e2 {{ Φ2 }} -∗
-               WP@{rs} interp_pair α β (e1,e2) {{ interp_tpair Φ1 Φ2 }}.
-  Proof.
-    iIntros "#Hctx H1 H2".
-    Opaque pairTV. iSimpl.
-    iApply (wp_bind _ (get_val _)).
-    { solve_proper. }
-    iApply (wp_wand with "H2").
-    iIntros (βv) "H2". iModIntro.
-    rewrite get_val_ITV. simpl.
-    iApply (wp_bind _ (get_val _)).
-    { solve_proper. }
-    iApply (wp_wand with "H1").
-    iIntros (αv) "H1". iModIntro.
-    rewrite get_val_ITV. simpl.
-    iApply wp_val.
-    iModIntro.
-    iExists αv,βv. iSplit; eauto with iFrame.
-  Qed.
-  Lemma compat_destruct {A1 A2 : ofe} (e1 : A1) (e2 : A2)
-    (Φ1 Φ2 Φ : ITV -n> iProp) (α : IT*IT*A2 -n> IT) (β : A1 -n> IT) :
-    heap_ctx ⊢ WP@{rs} β e1 {{ interp_tpair Φ1 Φ2 }} -∗
-               (∀ β1v β2v, protected Φ1 β1v -∗ protected Φ2 β2v -∗
-                      WP@{rs} α (IT_of_V β1v,IT_of_V β2v,e2) {{ Φ }}) -∗
-               WP@{rs} (interp_destruct β α (e1,e2)) {{ Φ }}.
-  Proof.
-    Local Opaque thunked thunkedV proj1T proj2T pairTV.
-    iIntros "#Hctx H1 H2".
-    iSimpl.
-    iApply wp_let.
-    iApply (wp_wand with "H1").
-    iIntros (βv) "H1". iModIntro.
-    iApply wp_let.
-    iApply (wp_alloc with "Hctx").
-    { solve_proper_please. }
-    iNext. iNext. iIntros (l1) "Hl1".
-    iApply (wp_val _ _ (thunkedV _ _)).
-    iModIntro. iSimpl.
-    iApply wp_let.
-    iApply (wp_alloc with "Hctx").
-    { solve_proper_please. }
-    iNext. iNext. iIntros (l2) "Hl2".
-    iApply (wp_val _ _ (thunkedV _ _)).
-    iModIntro. iSimpl.
-    iSimpl in "H1".
-    iDestruct "H1" as (βv1 βv2) "(#Hb & Hb1 & Hb2)".
-    iRewrite "Hb". iClear "Hb".
-    Local Transparent thunkedV thunked.
-    iApply ("H2" with "[Hb1 Hl1] [Hb2 Hl2]").
-    - simpl. iApply wp_lam. iNext.
-      simpl.
-      iApply (wp_bind _ (IFSCtx _ _)).
-      iApply (wp_read with "Hctx Hl1").
-      iNext. iNext. iIntros "Hl1".
-      iApply wp_val. iModIntro.
-      unfold IFSCtx. simpl.
-      rewrite IF_False; last lia.
-      iApply wp_seq.
-      { solve_proper. }
-      iApply (wp_write with "Hctx Hl1").
-      iNext. iNext. iIntros "Hl1".
-      rewrite proj1T_pairV. simpl.
-      repeat (iApply wp_tick; iNext).
-      by iApply wp_val.
-    - simpl. iApply wp_lam. iNext.
-      simpl.
-      iApply (wp_bind _ (IFSCtx _ _)).
-      iApply (wp_read with "Hctx Hl2").
-      iNext. iNext. iIntros "Hl2".
-      iApply wp_val. iModIntro.
-      unfold IFSCtx. simpl.
-      rewrite IF_False; last lia.
-      iApply wp_seq.
-      { solve_proper. }
-      iApply (wp_write with "Hctx Hl2").
-      iNext. iNext. iIntros "Hl2".
-      rewrite proj2T_pairV. simpl.
-      repeat (iApply wp_tick; iNext).
-      by iApply wp_val.
-  Qed.
-  Lemma compat_app {A1 A2 :ofe} (e1 : A1) (e2 : A2) Φ1 Φ2
-    (α : A1 -n> IT) (β : A2 -n> IT) :
-    heap_ctx ⊢ WP@{rs} α e1 {{ interp_tarr Φ1 Φ2 }} -∗
-               WP@{rs} β e2 {{ Φ1 }} -∗
-               WP@{rs} (interp_app α β (e1,e2)) {{ Φ2 }}.
-  Proof.
-    iIntros "#Hctx H1 H2".
-    iSimpl.
-    iApply (wp_bind _ (AppRSCtx _)).
-    iApply wp_let.
-    { solve_proper. }
-    iApply (wp_wand with "H2").
-    iIntros (βv) "H2".
-    iModIntro. iEval(cbn-[thunked]).
-    iApply (wp_alloc with "Hctx").
-    { solve_proper. }
-    iNext. iNext. iIntros (ℓ) "Hl".
-    iApply (wp_val _ _ (thunkedV _ _)).
-    iModIntro. unfold AppRSCtx.
-    iApply (wp_bind _ (AppLSCtx (IT_of_V (thunkedV (IT_of_V βv) ℓ)))).
-    { solve_proper. }
-    iApply (wp_wand with "H1").
-    iIntros (αv) "H1".
-    iModIntro. unfold AppLSCtx.
-    rewrite tv_into_val.
-    iApply ("H1" with "H2 Hl").
   Qed.
 
-  Lemma compat_lam {A : ofe} (e : A) (Φ1 Φ2 : ITV -n> iProp) (α : IT*A -n> IT) :
-    heap_ctx ⊢ (∀ βv, protected Φ1 βv -∗ WP@{rs} α (IT_of_V βv,e) {{ Φ2 }}) -∗
-               WP@{rs} (interp_lam α e) {{ interp_tarr Φ1 Φ2 }}.
+  (* Lemma compat_pair {A1 A2 : ofe} (e1 : A1) (e2 : A2) (Φ1 Φ2 : ITV -n> iProp) *)
+  (*   (α : A1 -n> IT) (β : A2 -n> IT) s : *)
+  (*   heap_ctx ⊢ WP@{rs} α e1 @ s {{ Φ1 }} -∗ *)
+  (*              WP@{rs} β e2 @ s {{ Φ2 }} -∗ *)
+  (*              WP@{rs} interp_pair α β (e1,e2) @ s {{ interp_tpair Φ1 Φ2 }}. *)
+  (* Proof. *)
+  (*   iIntros "#Hctx H1 H2". *)
+  (*   Opaque pairTV. iSimpl. *)
+  (*   iApply (wp_bind _ (get_val _)). *)
+  (*   { solve_proper. } *)
+  (*   iApply (wp_wand with "H2"). *)
+  (*   iIntros (βv) "H2". iModIntro. *)
+  (*   rewrite get_val_ITV. simpl. *)
+  (*   iApply (wp_bind _ (get_val _)). *)
+  (*   { solve_proper. } *)
+  (*   iApply (wp_wand with "H1"). *)
+  (*   iIntros (αv) "H1". iModIntro. *)
+  (*   rewrite get_val_ITV. simpl. *)
+  (*   iApply wp_val. *)
+  (*   iModIntro. *)
+  (*   iExists αv,βv. iSplit; eauto with iFrame. *)
+  (* Qed. *)
+  (* Lemma compat_destruct {A1 A2 : ofe} (e1 : A1) (e2 : A2) *)
+  (*   (Φ1 Φ2 Φ : ITV -n> iProp) (α : IT*IT*A2 -n> IT) (β : A1 -n> IT) s : *)
+  (*   heap_ctx ⊢ WP@{rs} β e1 @ s {{ interp_tpair Φ1 Φ2 }} -∗ *)
+  (*              (∀ β1v β2v, protected Φ1 β1v -∗ protected Φ2 β2v -∗ *)
+  (*                     WP@{rs} α (IT_of_V β1v,IT_of_V β2v,e2) @ s {{ Φ }}) -∗ *)
+  (*              WP@{rs} (interp_destruct β α (e1,e2)) @ s {{ Φ }}. *)
+  (* Proof. *)
+  (*   Local Opaque thunked thunkedV proj1T proj2T pairTV. *)
+  (*   iIntros "#Hctx H1 H2". *)
+  (*   iSimpl. *)
+  (*   iApply wp_let. *)
+  (*   iApply (wp_wand with "H1"). *)
+  (*   iIntros (βv) "H1". iModIntro. *)
+  (*   iApply wp_let. *)
+  (*   iApply (wp_alloc with "Hctx"). *)
+  (*   { solve_proper_please. } *)
+  (*   iNext. iNext. iIntros (l1) "Hl1". *)
+  (*   iApply (wp_val _ _ (thunkedV _ _)). *)
+  (*   iModIntro. iSimpl. *)
+  (*   iApply wp_let. *)
+  (*   iApply (wp_alloc with "Hctx"). *)
+  (*   { solve_proper_please. } *)
+  (*   iNext. iNext. iIntros (l2) "Hl2". *)
+  (*   iApply (wp_val _ _ (thunkedV _ _)). *)
+  (*   iModIntro. iSimpl. *)
+  (*   iSimpl in "H1". *)
+  (*   iDestruct "H1" as (βv1 βv2) "(#Hb & Hb1 & Hb2)". *)
+  (*   iRewrite "Hb". iClear "Hb". *)
+  (*   Local Transparent thunkedV thunked. *)
+  (*   iApply ("H2" with "[Hb1 Hl1] [Hb2 Hl2]"). *)
+  (*   - simpl. iApply wp_lam. iNext. *)
+  (*     simpl. *)
+  (*     iApply (wp_bind _ (IFSCtx _ _)). *)
+  (*     iApply (wp_read with "Hctx Hl1"). *)
+  (*     iNext. iNext. iIntros "Hl1". *)
+  (*     iApply wp_val. iModIntro. *)
+  (*     unfold IFSCtx. simpl. *)
+  (*     rewrite IF_False; last lia. *)
+  (*     iApply wp_seq. *)
+  (*     { solve_proper. } *)
+  (*     iApply (wp_write with "Hctx Hl1"). *)
+  (*     iNext. iNext. iIntros "Hl1". *)
+  (*     rewrite proj1T_pairV. simpl. *)
+  (*     repeat (iApply wp_tick; iNext). *)
+  (*     by iApply wp_val. *)
+  (*   - simpl. iApply wp_lam. iNext. *)
+  (*     simpl. *)
+  (*     iApply (wp_bind _ (IFSCtx _ _)). *)
+  (*     iApply (wp_read with "Hctx Hl2"). *)
+  (*     iNext. iNext. iIntros "Hl2". *)
+  (*     iApply wp_val. iModIntro. *)
+  (*     unfold IFSCtx. simpl. *)
+  (*     rewrite IF_False; last lia. *)
+  (*     iApply wp_seq. *)
+  (*     { solve_proper. } *)
+  (*     iApply (wp_write with "Hctx Hl2"). *)
+  (*     iNext. iNext. iIntros "Hl2". *)
+  (*     rewrite proj2T_pairV. simpl. *)
+  (*     repeat (iApply wp_tick; iNext). *)
+  (*     by iApply wp_val. *)
+  (* Qed. *)
+
+  Lemma compat_var {S} Ω τ (v : var S) :
+    typed_var Ω v τ →
+    ⊢ valid1 Ω (interp_var v) τ.
   Proof.
-    iIntros "#Hctx H".
+    iIntros (Hv ss) "Has #Hctx".
+    unfold ssubst_valid.
+    iInduction Hv as [|? ? ? Ω v] "IH" forall (ss); simpl.
+    - dependent elimination ss as [cons_ssubst αv ss].
+      simp list_of_tyctx list_of_ssubst interp_ssubst.
+      simp interp_var. simpl.
+      iDestruct "Has" as "[H _]".
+      by iApply wp_val.
+    - dependent elimination ss as [cons_ssubst αv ss].
+      simp list_of_tyctx list_of_ssubst interp_ssubst.
+      simp interp_var. simpl.
+      iDestruct "Has" as "[_ H]".
+      iApply ("IH" with "H").
+  Qed.
+
+  Lemma compat_app {S1 S2} (Ω1 : tyctx S1) (Ω2 : tyctx S2)
+    α β τ1 τ2 :
+    ⊢ valid1 Ω1 α (tArr τ1 τ2) -∗
+      valid1 Ω2 β τ1 -∗
+      valid1 (tyctx_app Ω1 Ω2) (interp_app α β ◎ interp_scope_split) τ2.
+  Proof.
+    iIntros "H1 H2".
+    iIntros (αs) "Has #Hctx".
+    iEval(cbn-[interp_app]).
+    rewrite ctx_valid_split.
+    destruct (interp_ty_ctx_split αs) as [a1 a2].
+    iDestruct "Has" as "[Ha1 Ha2]". cbn-[interp_app].
+    iSpecialize ("H1" with "Ha1 Hctx").
+    iSpecialize ("H2" with "Ha2 Hctx").
+    Local Opaque Thunk.
+    iSimpl.
+    iApply wp_let.
+    iApply (wp_wand with "H2").
+    iIntros (βv) "H2".
+    iModIntro. iSimpl.
+    iApply wp_let.
+    iApply (wp_wand with "H1").
+    iIntros (αv) "H1".
+    iModIntro. iSimpl.
+    by iApply "H1".
+  Qed.
+
+  Lemma compat_lam Ω τ1 τ2 α :
+    ⊢ valid1 (τ1::Ω) α τ2 -∗
+      valid1 Ω (interp_lam α) (tArr τ1 τ2).
+  Proof.
+    iIntros "H".
+    iIntros (αs) "Has #Hctx".
     iApply wp_val.
-    iModIntro.
-    iIntros (βv l) "Hb Hl".
+    iModIntro. simpl.
+    iIntros (βv) "Hb".
+    iApply (wp_bind _ (AppRSCtx _)).
+    Local Transparent Thunk.
+    Local Opaque thunked thunkedV.
+    iSimpl. iApply (wp_alloc with "Hctx").
+    { solve_proper. }
+    iNext. iNext. iIntros (l) "Hl".
+    iApply wp_val. iModIntro.
+    unfold AppRSCtx.
     iApply wp_lam. iNext.
     iEval(cbn-[thunked]).
-    iAssert (thunked (IT_of_V βv) l ≡ IT_of_V (thunkedV (IT_of_V βv) l))%I as "Hth".
-    { rewrite tv_into_val. done. }
-    iRewrite "Hth". iClear "Hth".
-    iApply ("H" with "[-]").
-    simpl. iApply wp_lam. iNext.
+    iApply ("H" with "[-] Hctx").
+    iSimpl. iFrame "Has".
+    iExists _.
+    rewrite IT_to_of_V. iSplit; eauto.
+    Local Transparent thunked thunkedV.
+    iApply wp_lam. iNext. simpl.
     iApply (wp_bind _ (IFSCtx _ _)).
     iApply (wp_read with "Hctx Hl").
     iNext. iNext. iIntros "Hl".
@@ -249,64 +384,12 @@ Section affine.
     iApply "Hb".
   Qed.
 
-  Inductive expr : scope → Type :=
-  | Val {S} : val S → expr S
-  | AffApp {S1 S2} : expr S1 → expr S2 → expr (S1++S2)
-  (* | EPair {S} : expr S → expr S → expr S *)
-  (* | EDestruct {S} : expr S → expr (()::()::S) → expr S *)
-  | EEmbed {S} : input_lang.lang.expr S → expr S
-  with val : scope → Type :=
-  | LitBool (b : bool) {S} : val S
-  | LitNat (n : nat) {S} : val S
-  | LitUnit {S} : val S
-  (* | VPair {S} : val S → val S → val S *)
-  | VLam {S} : expr (tt::S) → val S
-  | Var {S} : var S → val S.
-
-  Definition split_scope {S1 S2} : interp_scope rs (S1++S2) -n> prodO (interp_scope rs S1) (interp_scope rs S2).
-  Proof.
-    induction S1 as [|? S1]; simpl.
-    - simple refine (λne x, (tt, x)).
-      solve_proper.
-    - simple refine (λne xy, let ss := IHS1 xy.2 in ((xy.1, ss.1), ss.2)).
-      solve_proper.
-  Qed.
-
-  Program Definition interp_var {S} (v : var S) : interp_scope rs S -n> IT :=
-    λne env, interp_var rs v env ⊙ (Nat 0).
-  Solve All Obligations with solve_proper.
-
-  Fixpoint interp_expr {S} (e : expr S) : interp_scope rs S -n> IT :=
-    match e with
-    | Val v => interp_val v
-    | AffApp e1 e2 => interp_app (interp_expr e1) (interp_expr e2) ◎ split_scope
-    | EEmbed ei => input_lang.interp.interp_expr rs ei
-    end
-  with interp_val {S} (v : val S) : interp_scope rs S -n> IT :=
-    match v with
-    | LitBool b => interp_litbool b
-    | LitNat n  => interp_litnat n
-    | LitUnit   => interp_litunit
-    | Var v     => interp_var v
-    | VLam e    => interp_lam (interp_expr e)
-    end.
-
-  Inductive ty_conv : ty → input_lang.lang.ty → Type :=
-  | ty_conv_bool : ty_conv tBool Tnat
-  | ty_conv_int  : ty_conv tInt  Tnat
-  | ty_conv_unit : ty_conv tUnit Tnat
-  | ty_conv_fun {τ1 τ2 t1 t2} :
-    ty_conv τ1 t1 → ty_conv τ2 t2 →
-    ty_conv (tArr τ1 τ2) (Tarr (Tarr Tnat t1) t2)
-  .
 
   Program Definition glue1_fun (glue1 glue2 : IT -n> IT) : IT -n> IT := λne α,
-    λit x, LET (glue2 (Force x)) $ λne x,
+    λit xthnk,
+      LET (Force xthnk) $ λne x,
+      LET (glue2 x) $ λne x,
       LET (α ⊙ (Thunk x)) glue1.
-  Solve All Obligations with solve_proper_please.
-  Program Definition glue2_fun (glue1 glue2 : IT -n> IT) : IT -n> IT := λne α,
-    λit x, LET (glue1 (Force x)) $ λne x,
-      LET (α ⊙ (Thunk x)) glue2.
   Solve All Obligations with solve_proper_please.
 
   Program Definition glue2_bool : IT -n> IT := λne α,
@@ -324,5 +407,200 @@ Section affine.
     | ty_conv_bool => glue2_bool
     | ty_conv_int  => idfun
     | ty_conv_unit => constO (Nat 0)
-    | ty_conv_fun conv1 conv2 => glue2_fun (glue1 conv1) (glue2 conv2)
+    | ty_conv_fun conv1 conv2 => glue1_fun (glue1 conv1) (glue2 conv2)
     end.
+
+ 
+  Lemma compat_glue_fun (αv : ITV) (glue1 glue2 : IT -n> IT) (Φ1 Φ2 Φ1' Φ2' : ITV -n> iProp) :
+    heap_ctx ⊢
+      (∀ βv, Φ1 βv -∗ WP@{rs} glue1 (IT_of_V βv) @ s {{ x, □ Φ1' x }}) -∗
+      (∀ βv, Φ2' βv -∗ WP@{rs} glue2 (IT_of_V βv) @ s {{ Φ2 }}) -∗
+      (* (unit  →  τ1') → τ2' *)
+      □ (∀ βv, □ (WP@{rs} IT_of_V βv ⊙ (Nat 0) @ s {{ Φ1' }}) -∗
+             WP@{rs} IT_of_V αv ⊙ (IT_of_V βv) @ s {{ Φ2' }}) -∗
+      WP@{rs} glue1_fun glue2 glue1 (IT_of_V αv) @ s {{ interp_tarr Φ1 Φ2 }}.
+   Proof.
+     iIntros "#Hctx G1 G2 #H1".
+     iApply wp_val. iModIntro.
+     iIntros (βv) "Hb".
+     Local Opaque thunked thunkedV.
+     iSimpl. iApply (wp_bind _ (AppRSCtx _)).
+     iApply (wp_alloc with "Hctx").
+     { solve_proper. }
+     iNext. iNext. iIntros (l) "Hl".
+     iApply wp_val. iModIntro.
+     unfold AppRSCtx.
+     iApply wp_lam. iNext.
+     iEval(cbn-[thunked]).
+     iApply wp_let.
+     { solve_proper. }
+     iApply wp_lam.
+     (* forcing a thunk *)
+     iNext. iSimpl.
+     iApply (wp_bind _ (IFSCtx _ _)).
+     { solve_proper. }
+     iApply (wp_read with "Hctx Hl").
+     iNext. iNext. iIntros "Hl".
+     iApply wp_val. iModIntro.
+     unfold IFSCtx. simpl.
+     rewrite IF_False; last lia.
+     iApply wp_seq.
+     { solve_proper. }
+     iApply (wp_write with "Hctx Hl").
+     iNext. iNext. iIntros "Hl".
+     iApply wp_val. iModIntro.
+     (* doing the glue for the argument *)
+     iApply (wp_let).
+     { solve_proper. }
+     iSpecialize ("G1" with "Hb").
+     iApply (wp_wand with "G1").
+     iIntros (β'v) "#Hb". iModIntro.
+     iSimpl.
+     (* calling the original function *)
+     iApply wp_let.
+     { solve_proper. }
+     iApply (wp_bind _ (AppRSCtx _)).
+     { solve_proper. }
+     iApply (wp_alloc with "Hctx").
+     { solve_proper. }
+     iNext. iNext. iIntros (l') "Hl'".
+     iApply wp_val. iModIntro.
+     unfold AppRSCtx.
+     iClear "Hl". clear l.
+     iApply fupd_wp.
+     { solve_proper. }
+     iMod (inv_alloc (nroot.@"yolo") _ (∃ n, pointsto l' (Nat n)) with "[Hl']") as "#Hinv".
+     { iNext. iExists _; done. }
+     iSpecialize ("H1" $! (thunkedV (IT_of_V β'v) l') with "[-G2]").
+     { iModIntro.
+       iApply wp_lam. iNext. iSimpl.
+       iApply (wp_bind _ (IFSCtx _ _)).
+       iApply (wp_read_atomic _ _ (⊤∖ nclose (nroot.@"storeE")) with "Hctx").
+       { set_solver. }
+       iInv (nroot.@"yolo") as (n) "Hl'" "Hcl".
+       iModIntro. iExists (Nat n). iFrame.
+       iNext. iNext. iIntros "Hl'".
+       iMod ("Hcl" with "[Hl']") as "_".
+       { iNext. eauto with iFrame. }
+       iModIntro. iApply wp_val.
+       iModIntro.
+       unfold IFSCtx. simpl.
+       destruct n as [|n].
+       - rewrite IF_False; last lia.
+         iApply wp_seq.
+         { solve_proper. }
+         iApply (wp_write_atomic _ _ (⊤∖ nclose (nroot.@"storeE")) with "Hctx").
+         { set_solver. }
+         iInv (nroot.@"yolo") as (n) "Hl'" "Hcl".
+         iModIntro. iExists (Nat n). iFrame.
+         iNext. iNext. iIntros "Hl'".
+         iMod ("Hcl" with "[Hl']") as "_".
+         { iNext. eauto with iFrame. }
+         iModIntro. iApply wp_val.
+         iModIntro. done.
+       - rewrite IF_True; last lia.
+         iApply wp_err. done. }
+     iModIntro.
+     iApply (wp_wand with "H1").
+     iIntros (γv) "H2".
+     iModIntro.
+     by iApply "G2".
+  Qed.
+
+  Lemma compat_glue2_fun (αv : ITV) (glue1 glue2 : IT -n> IT) (Φ1 Φ2 Φ1' Φ2' : ITV -n> iProp) A :
+    heap_ctx ⊢
+      □ (∀ βv, Φ1' βv -∗ WP@{rs} glue1 (IT_of_V βv) @ s {{ Φ1 }}) -∗
+      □ (∀ βv, Φ2 βv -∗ WP@{rs} glue2 (IT_of_V βv) @ s {{ x, □ Φ2' x }}) -∗
+      □ (A -∗ interp_tarr Φ1 Φ2 αv) -∗
+      (WP@{rs} glue1_fun glue2 glue1 (IT_of_V αv) @ s {{ αv,
+            (* av : (unit →  τ1') → τ2' *)
+            □ (∀ βv, □ (WP@{rs} IT_of_V βv ⊙ (Nat 0) @ s {{ Φ1' }}) -∗
+                     WP@{rs} IT_of_V αv ⊙ (IT_of_V βv) @ s {{ Φ2' }}) }}).
+   Proof.
+     iIntros "#Hctx #G1 #G2 #H1 HA".
+     iApply wp_val. iModIntro.
+     iSpecialize ("H1" with "HA").
+     iIntros (βv) "Hb".
+     Local Opaque thunked thunkedV.
+     iSimpl. iApply (wp_bind _ (AppRSCtx _)).
+     iApply (wp_alloc with "Hctx").
+     { solve_proper. }
+     iNext. iNext. iIntros (l) "Hl".
+     iApply wp_val. iModIntro.
+     unfold AppRSCtx.
+     iApply wp_lam. iNext.
+     iEval(cbn-[thunked]).
+     iApply wp_let.
+     { solve_proper. }
+     iApply wp_lam.
+     (* forcing a thunk *)
+     iNext. iSimpl.
+     iApply (wp_bind _ (IFSCtx _ _)).
+     { solve_proper. }
+     iApply (wp_read with "Hctx Hl").
+     iNext. iNext. iIntros "Hl".
+     iApply wp_val. iModIntro.
+     unfold IFSCtx. simpl.
+     rewrite IF_False; last lia.
+     iApply wp_seq.
+     { solve_proper. }
+     iApply (wp_write with "Hctx Hl").
+     iNext. iNext. iIntros "Hl".
+     iApply wp_val. iModIntro.
+     (* doing the glue for the argument *)
+     iApply (wp_let).
+     { solve_proper. }
+     iSpecialize ("G1" with "Hb").
+     iApply (wp_wand with "G1").
+     iIntros (β'v) "#Hb". iModIntro.
+     iSimpl.
+     (* calling the original function *)
+     iApply wp_let.
+     { solve_proper. }
+     iApply (wp_bind _ (AppRSCtx _)).
+     { solve_proper. }
+     iApply (wp_alloc with "Hctx").
+     { solve_proper. }
+     iNext. iNext. iIntros (l') "Hl'".
+     iApply wp_val. iModIntro.
+     unfold AppRSCtx.
+     iClear "Hl". clear l.
+     iApply fupd_wp.
+     { solve_proper. }
+     iMod (inv_alloc (nroot.@"yolo") _ (∃ n, pointsto l' (Nat n)) with "[Hl']") as "#Hinv".
+     { iNext. iExists _; done. }
+     iSpecialize ("H1" $! (thunkedV (IT_of_V β'v) l') with "[-G2]").
+     { iModIntro.
+       iApply wp_lam. iNext. iSimpl.
+       iApply (wp_bind _ (IFSCtx _ _)).
+       iApply (wp_read_atomic _ _ (⊤∖ nclose (nroot.@"storeE")) with "Hctx").
+       { set_solver. }
+       iInv (nroot.@"yolo") as (n) "Hl'" "Hcl".
+       iModIntro. iExists (Nat n). iFrame.
+       iNext. iNext. iIntros "Hl'".
+       iMod ("Hcl" with "[Hl']") as "_".
+       { iNext. eauto with iFrame. }
+       iModIntro. iApply wp_val.
+       iModIntro.
+       unfold IFSCtx. simpl.
+       destruct n as [|n].
+       - rewrite IF_False; last lia.
+         iApply wp_seq.
+         { solve_proper. }
+         iApply (wp_write_atomic _ _ (⊤∖ nclose (nroot.@"storeE")) with "Hctx").
+         { set_solver. }
+         iInv (nroot.@"yolo") as (n) "Hl'" "Hcl".
+         iModIntro. iExists (Nat n). iFrame.
+         iNext. iNext. iIntros "Hl'".
+         iMod ("Hcl" with "[Hl']") as "_".
+         { iNext. eauto with iFrame. }
+         iModIntro. iApply wp_val.
+         iModIntro. done.
+       - rewrite IF_True; last lia.
+         iApply wp_err. done. }
+     iModIntro.
+     iApply (wp_wand with "H1").
+     iIntros (γv) "H2".
+     iModIntro.
+     by iApply "G2".
+   Qed.
