theories/lang_generic.v
@@ -1,0 +1,90 @@
+From gitrees Require Import prelude.
+From gitrees Require Import gitree.
+From Equations Require Import Equations.
+Require Import List.
+Import ListNotations.
+
+(** XXX: We /NEED/ this line for [Equations Derive] to work,
+ this flag is globally unset by std++, but Equations need obligations to be transparent. *)
+Set Transparent Obligations.
+
+Derive NoConfusion NoConfusionHom for list.
+
+Definition scope := (list unit).
+
+(** Variables in a context *)
+Inductive var : scope → Type :=
+| Vz : forall {S : scope} {s}, var (s::S)
+| Vs : forall {S : scope} {s}, var S -> var (s::S)
+.
+Derive Signature NoConfusion for var.
+
+Inductive tyctx (ty : Type) : scope → Type :=
+| empC : tyctx ty []
+| consC : forall{Γ}, ty → tyctx ty Γ → tyctx ty (()::Γ)
+.
+Arguments empC {_}.
+Arguments consC {_ _} _ _.
+
+Equations list_of_tyctx {S ty} (Γ : tyctx ty S) : list ty :=
+  list_of_tyctx empC := [];
+  list_of_tyctx (consC τ Γ') := τ::list_of_tyctx Γ'.
+
+Equations tyctx_app {S1 S2 ty} (c1 : tyctx ty S1) (c2 : tyctx ty S2) : tyctx ty (S1++S2) :=
+  tyctx_app empC         c2 := c2;
+  tyctx_app (consC τ c1) c2 := consC τ (tyctx_app c1 c2).
+
+Inductive typed_var {ty : Type}: forall {S}, tyctx ty S → var S → ty → Prop :=
+| typed_var_Z S (τ : ty) (Γ : tyctx ty S) :
+  typed_var (consC τ Γ) Vz τ
+| typed_var_S S (τ τ' : ty) (Γ : tyctx ty S) v :
+  typed_var Γ v τ →
+  typed_var (consC τ' Γ) (Vs v) τ
+.
+
+Section interp.
+  Context {E: opsInterp}.
+  Notation IT := (IT E).
+  Notation ITV := (ITV E).
+
+  Fixpoint interp_scope (S : scope) : ofe :=
+    match S with
+    | [] => unitO
+    | τ::Sc => prodO IT (interp_scope Sc)
+    end.
+
+  Instance interp_scope_cofe S : Cofe (interp_scope S).
+  Proof. induction S; simpl; apply _. Qed.
+
+  Instance interp_scope_inhab S : Inhabited (interp_scope S).
+  Proof. induction S; simpl; apply _. Defined.
+
+  Equations interp_var {S : scope} (v : var S) : interp_scope S -n> IT :=
+    interp_var (S:=(_::_))     Vz := fstO;
+    interp_var (S:=(_::Sc)) (Vs v) := interp_var v ◎ sndO.
+
+  Instance interp_var_ne S (v : var S) : NonExpansive (@interp_var S v).
+  Proof.
+    intros n D1 D2 HD12. induction v; simp interp_var.
+    - by f_equiv.
+    - eapply IHv. by f_equiv.
+  Qed.
+
+  Global Instance interp_var_proper S (v : var S) : Proper ((≡) ==> (≡)) (interp_var v).
+  Proof. apply ne_proper. apply _. Qed.
+
+  (** scope substituions *)
+  Inductive ssubst : scope → Type :=
+  | emp_ssubst : ssubst []
+  | cons_ssubst {S} : ITV → ssubst S → ssubst (()::S)
+  .
+
+  Equations interp_ssubst {S} (ss : ssubst S) : interp_scope S :=
+    interp_ssubst emp_ssubst := ();
+    interp_ssubst (cons_ssubst αv ss) := (IT_of_V αv, interp_ssubst ss).
+
+  Equations list_of_ssubst {S} (ss : ssubst S) : list ITV :=
+    list_of_ssubst emp_ssubst := [];
+    list_of_ssubst (cons_ssubst αv ss) := αv::(list_of_ssubst ss).
+
+End interp.
